fstar/Hacspec.Lib.Nat.fst
@@ -4,4 +4,6 @@ open Hacspec.Lib.Int
 
 let nat_mod (n: nat) = x:nat{x < n}
 
-assume val from_secret_literal (#n: nat) (x:uint128) : nat_mod n
+assume val from_secret_literal (x:uint128) : n:nat{v x == n}
+
+let pow2 (x: nat) : nat = pow2 x
